clean up
add hb actions to make connection to paper clearer

misc/array-map.bpl
@@ -195,10 +195,8 @@ function {:inline} {:linear "this"} TidCollector(x: Invoc) : [Invoc]bool
 
 // ---------- Representation of execution and linearization
 
-// hb(x, y) : x happens-before y.  // TODO make var, have actions to add these
-// We assume there exists such a function, given by the client program
-function hb(x: Invoc, y: Invoc) : bool;
-axiom (forall n: Invoc :: !hb(n, n));
+// hb[x][y] : x happens-before y.
+var {:layer 1,2} hb: [Invoc][Invoc]bool;
 
 // A shared global variable that builds the linearization
 var {:layer 1,2} lin: SeqInvoc;
@@ -227,11 +225,30 @@ procedure {:layer 1} intro_writeVis(n: Invoc, s: SetInvoc)
 procedure {:layer 1} {:inline 1} intro_writeLin(n: Invoc)
   requires {:layer 1} !Seq_elem(n, lin);
   // To show that linearization is consistent with happens-before
-  requires {:layer 1} (forall n1 : Invoc :: hb(n1, n) ==> Seq_elem(n1, lin));
+  requires {:layer 1} (forall n1 : Invoc :: hb[n1][n] ==> Seq_elem(n1, lin));
   ensures {:layer 1} Seq_elem(n, lin);
   modifies lin;
 {
   lin := Seq_append(lin, n);
+}
+
+procedure {:layer 1} {:inline 1} intro_writeHb(n1: Invoc, n2: Invoc)
+  modifies hb;
+{
+  hb[n1] := hb[n1][n2 := true];
+}
+
+
+// ---------- Consistency levels
+
+function {:inline} Consistency.absolute(hb: [Invoc]SetInvoc, lin: SeqInvoc,
+    vis: [Invoc]SetInvoc, n: Invoc, n_vis: SetInvoc): bool {
+  n_vis == Set_ofSeq(lin)
+}
+
+function {:inline} Consistency.monotonic(hb: [Invoc]SetInvoc, lin: SeqInvoc,
+    vis: [Invoc]SetInvoc, n: Invoc, n_vis: SetInvoc): bool {
+  (forall i: Invoc :: hb[i][n] ==> Set_subset(vis[i], n_vis))
 }
 
 
@@ -311,7 +328,11 @@ procedure {:layer 1} lemma_state_Set_union(k: int, s, t: SetInvoc);
 
 // ---------- Atomic specification program:
 
-// procedure {:atomic} {:layer 2} hb_action(n1: Invoc, n2: Invoc)
+procedure {:atomic} {:layer 2} hb_action_atomic(n1: Invoc, n2: Invoc)
+  modifies hb;
+{
+  hb[n1] := hb[n1][n2 := true];
+}
 
 procedure {:atomic} {:layer 2} put_call_atomic({:linear "this"} this: Invoc) {}
 
@@ -324,9 +345,7 @@ procedure {:atomic} {:layer 2} put_spec(k: int, v: int, {:linear "this"} this: I
   assume true;
   abs[k] := v;
 
-  // Is absolute
-  // assume my_vis == Set_ofSeq(lin);
-  my_vis := Set_ofSeq(lin);
+  assume Consistency.absolute(hb, lin, vis, this, my_vis);
 
   lin := Seq_append(lin, this);
   vis[this] := my_vis;
@@ -344,9 +363,7 @@ procedure {:atomic} {:layer 2} get_spec(k: int, {:linear "this"} this: Invoc) re
   // Get satisfies its functional spec
   v := abs[k];
 
-  // Get is absolute
-  // assume my_vis == Set_ofSeq(lin);
-  my_vis := Set_ofSeq(lin);
+  assume Consistency.absolute(hb, lin, vis, this, my_vis);
 
   lin := Seq_append(lin, this);
   vis[this] := my_vis;
@@ -373,8 +390,7 @@ procedure {:atomic} {:layer 2} contains_spec(v: int, {:linear "this"} this: Invo
   // Contains satisfies its functional spec
   assume contains_func_spec(my_vis, lin, witness_k, v, res);
 
-  // Contains is monotonic
-  assume (forall j: Invoc :: hb(j, this) ==> Set_subset(vis[j], my_vis));
+  assume Consistency.monotonic(hb, lin, vis, this, my_vis);
 
   lin := Seq_append(lin, this);
   vis[this] := my_vis;
@@ -413,7 +429,7 @@ function {:inline} abstracts(conc: [int]int, abs: Map.State) : bool
 
 // The invariants
 function {:inline} tableInv(table: [int]int, abs: Map.State, tabvis: [int]SetInvoc,
-                            lin: SeqInvoc, vis: [Invoc]SetInvoc, tabLen: int,
+                            hb: [Invoc][Invoc]bool, lin: SeqInvoc, vis: [Invoc]SetInvoc, tabLen: int,
                             called: [Invoc]bool, returned: [Invoc]bool) : bool
 {
   abstracts(table, abs)
@@ -439,7 +455,7 @@ function {:inline} tableInv(table: [int]int, abs: Map.State, tabvis: [int]SetInv
   && (forall n1, n2: Invoc :: {vis[n2][n1]}
     vis[n2][n1] && returned[n2] ==> Set_ofSeq(lin)[n1])
   // Used to infer that invocations don't modify vis after they've returned
-  && (forall n1, n2 : Invoc :: called[n1] && hb(n2, n1) ==> returned[n2])
+  && (forall n1, n2 : Invoc :: called[n1] && hb[n2][n1] ==> returned[n2])
   // To establish precondition of intro_writeLin
   && (forall n: Invoc :: returned[n] ==> Seq_elem(n, lin))
 }
@@ -513,41 +529,50 @@ procedure {:layer 1} {:inline 1} intro_writeReturned({:linear "this"} this: Invo
 // ---------- Implementation of Map:
 
 
+procedure {:yields} {:layer 1} {:refines "hb_action_atomic"}
+    hb_action(n1: Invoc, n2: Invoc)
+  requires {:layer 1} returned[n1] && !called[n2];
+{
+  call intro_writeHb(n1, n2);
+  yield;
+}
+
+
 procedure {:yields} {:layer 1} {:refines "put_call_atomic"}
     put_call({:linear "this"} this: Invoc)
-  requires {:layer 1} tableInv(table, abs, tabvis, lin, vis, tabLen, called, returned);
+  requires {:layer 1} tableInv(table, abs, tabvis, hb, lin, vis, tabLen, called, returned);
   // everything before this has returned
-  requires {:layer 1} (forall n1: Invoc :: hb(n1, this) ==> returned[n1]);
+  requires {:layer 1} (forall n1: Invoc :: hb[n1][this] ==> returned[n1]);
   // this has not been called or returned yet
   requires {:layer 1} (!called[this] && !returned[this]);
-  ensures {:layer 1} tableInv(table, abs, tabvis, lin, vis, tabLen, called, returned);
+  ensures {:layer 1} tableInv(table, abs, tabvis, hb, lin, vis, tabLen, called, returned);
   ensures {:layer 1} preLP(called, returned, lin, this);
   modifies called;
 {
   yield;
-  assert {:layer 1} tableInv(table, abs, tabvis, lin, vis, tabLen, called, returned);
-  assert {:layer 1} (forall n1: Invoc :: hb(n1, this) ==> returned[n1]);
+  assert {:layer 1} tableInv(table, abs, tabvis, hb, lin, vis, tabLen, called, returned);
+  assert {:layer 1} (forall n1: Invoc :: hb[n1][this] ==> returned[n1]);
   assert {:layer 1} (!called[this] && !returned[this]);
 
   call intro_writeCalled(this);
   yield;
-  assert {:layer 1} tableInv(table, abs, tabvis, lin, vis, tabLen, called, returned);
+  assert {:layer 1} tableInv(table, abs, tabvis, hb, lin, vis, tabLen, called, returned);
   assert {:layer 1} preLP(called, returned, lin, this);
 }
 
 
 procedure {:yields} {:layer 1} {:refines "put_spec"} put(k, v: int, {:linear "this"} this: Invoc)
-  requires {:layer 1} tableInv(table, abs, tabvis, lin, vis, tabLen, called, returned);
+  requires {:layer 1} tableInv(table, abs, tabvis, hb, lin, vis, tabLen, called, returned);
   requires {:layer 1} preLP(called, returned, lin, this);
   requires {:layer 1} invoc_m(this) == Map.put && invoc_k(this) == k && invoc_v(this) == v;
   requires {:layer 1} 0 <= k && k < tabLen;
-  ensures {:layer 1} tableInv(table, abs, tabvis, lin, vis, tabLen, called, returned);
+  ensures {:layer 1} tableInv(table, abs, tabvis, hb, lin, vis, tabLen, called, returned);
   ensures {:layer 1} postLP(called, returned, lin, this);
   ensures {:layer 1} (forall n1: Invoc :: {vis[this][n1]}
     vis[this][n1] ==> Set_ofSeq(lin)[n1]);
 {
   var {:layer 1} my_vis: SetInvoc;
-  yield; assert {:layer 1} tableInv(table, abs, tabvis, lin, vis, tabLen, called, returned) && preLP(called, returned, lin, this);
+  yield; assert {:layer 1} tableInv(table, abs, tabvis, hb, lin, vis, tabLen, called, returned) && preLP(called, returned, lin, this);
 
   call writeTable(k, v);
 
@@ -557,7 +582,7 @@ procedure {:yields} {:layer 1} {:refines "put_spec"} put(k, v: int, {:linear "th
   call intro_writeVis(this, my_vis);
   call intro_writeAbs(k, v);
 
-  yield; assert {:layer 1} tableInv(table, abs, tabvis, lin, vis, tabLen, called, returned)
+  yield; assert {:layer 1} tableInv(table, abs, tabvis, hb, lin, vis, tabLen, called, returned)
     && postLP(called, returned, lin, this);
   assert {:layer 1} (forall n1: Invoc :: {vis[this][n1]}
     vis[this][n1] ==> Set_ofSeq(lin)[n1]);
@@ -565,15 +590,15 @@ procedure {:yields} {:layer 1} {:refines "put_spec"} put(k, v: int, {:linear "th
 
 procedure {:yields} {:layer 1} {:refines "put_return_atomic"}
     put_return({:linear "this"} this: Invoc)
-  requires {:layer 1} tableInv(table, abs, tabvis, lin, vis, tabLen, called, returned);
+  requires {:layer 1} tableInv(table, abs, tabvis, hb, lin, vis, tabLen, called, returned);
   requires {:layer 1} postLP(called, returned, lin, this);
   requires {:layer 1} (forall n1: Invoc :: {vis[this][n1]}
     vis[this][n1] ==> Set_ofSeq(lin)[n1]);
-  ensures {:layer 1} tableInv(table, abs, tabvis, lin, vis, tabLen, called, returned);
+  ensures {:layer 1} tableInv(table, abs, tabvis, hb, lin, vis, tabLen, called, returned);
   modifies returned;
 {
   yield;
-  assert {:layer 1} tableInv(table, abs, tabvis, lin, vis, tabLen, called, returned);
+  assert {:layer 1} tableInv(table, abs, tabvis, hb, lin, vis, tabLen, called, returned);
   assert {:layer 1} postLP(called, returned, lin, this);
   assert {:layer 1} (forall n1: Invoc :: {vis[this][n1]}
     vis[this][n1] ==> Set_ofSeq(lin)[n1]);
@@ -581,45 +606,45 @@ procedure {:yields} {:layer 1} {:refines "put_return_atomic"}
   call intro_writeReturned(this);
 
   yield;
-  assert {:layer 1} tableInv(table, abs, tabvis, lin, vis, tabLen, called, returned);
+  assert {:layer 1} tableInv(table, abs, tabvis, hb, lin, vis, tabLen, called, returned);
 }
 
 
 procedure {:yields} {:layer 1} {:refines "get_call_atomic"}
     get_call({:linear "this"} this: Invoc)
-  requires {:layer 1} tableInv(table, abs, tabvis, lin, vis, tabLen, called, returned);
+  requires {:layer 1} tableInv(table, abs, tabvis, hb, lin, vis, tabLen, called, returned);
   // everything before this has returned
-  requires {:layer 1} (forall n1: Invoc :: hb(n1, this) ==> returned[n1]);
+  requires {:layer 1} (forall n1: Invoc :: hb[n1][this] ==> returned[n1]);
   // this has not been called or returned yet
   requires {:layer 1} (!called[this] && !returned[this]);
-  ensures {:layer 1} tableInv(table, abs, tabvis, lin, vis, tabLen, called, returned);
+  ensures {:layer 1} tableInv(table, abs, tabvis, hb, lin, vis, tabLen, called, returned);
   ensures {:layer 1} preLP(called, returned, lin, this);
   modifies called;
 {
   yield;
-  assert {:layer 1} tableInv(table, abs, tabvis, lin, vis, tabLen, called, returned);
-  assert {:layer 1} (forall n1: Invoc :: hb(n1, this) ==> returned[n1]);
+  assert {:layer 1} tableInv(table, abs, tabvis, hb, lin, vis, tabLen, called, returned);
+  assert {:layer 1} (forall n1: Invoc :: hb[n1][this] ==> returned[n1]);
   assert {:layer 1} (!called[this] && !returned[this]);
 
   call intro_writeCalled(this);
   yield;
-  assert {:layer 1} tableInv(table, abs, tabvis, lin, vis, tabLen, called, returned);
+  assert {:layer 1} tableInv(table, abs, tabvis, hb, lin, vis, tabLen, called, returned);
   assert {:layer 1} preLP(called, returned, lin, this);
 }
 
 procedure {:yields} {:layer 1} {:refines "get_spec"} get(k: int, {:linear "this"} this: Invoc)
   returns (v: int)
-  requires {:layer 1} tableInv(table, abs, tabvis, lin, vis, tabLen, called, returned);
+  requires {:layer 1} tableInv(table, abs, tabvis, hb, lin, vis, tabLen, called, returned);
   requires {:layer 1} preLP(called, returned, lin, this);
   requires {:layer 1} invoc_m(this) == Map.get && invoc_k(this) == k;
   requires {:layer 1} 0 <= k && k < tabLen;
-  ensures {:layer 1} tableInv(table, abs, tabvis, lin, vis, tabLen, called, returned);
+  ensures {:layer 1} tableInv(table, abs, tabvis, hb, lin, vis, tabLen, called, returned);
   ensures {:layer 1} postLP(called, returned, lin, this);
   ensures {:layer 1} (forall n1: Invoc :: {vis[this][n1]}
     vis[this][n1] ==> Set_ofSeq(lin)[n1]);
 {
   var {:layer 1} my_vis: SetInvoc;
-  yield; assert {:layer 1} tableInv(table, abs, tabvis, lin, vis, tabLen, called, returned) && preLP(called, returned, lin, this);
+  yield; assert {:layer 1} tableInv(table, abs, tabvis, hb, lin, vis, tabLen, called, returned) && preLP(called, returned, lin, this);
 
   call v := readTable(k);
 
@@ -627,7 +652,7 @@ procedure {:yields} {:layer 1} {:refines "get_spec"} get(k: int, {:linear "this"
   call intro_writeVis(this, my_vis);
   call intro_writeLin(this);
 
-  yield; assert {:layer 1} tableInv(table, abs, tabvis, lin, vis, tabLen, called, returned)
+  yield; assert {:layer 1} tableInv(table, abs, tabvis, hb, lin, vis, tabLen, called, returned)
     && postLP(called, returned, lin, this);
   assert {:layer 1} (forall n1: Invoc :: {vis[this][n1]}
     vis[this][n1] ==> Set_ofSeq(lin)[n1]);
@@ -635,15 +660,15 @@ procedure {:yields} {:layer 1} {:refines "get_spec"} get(k: int, {:linear "this"
 
 procedure {:yields} {:layer 1} {:refines "get_return_atomic"}
     get_return({:linear "this"} this: Invoc)
-  requires {:layer 1} tableInv(table, abs, tabvis, lin, vis, tabLen, called, returned);
+  requires {:layer 1} tableInv(table, abs, tabvis, hb, lin, vis, tabLen, called, returned);
   requires {:layer 1} postLP(called, returned, lin, this);
   requires {:layer 1} (forall n1: Invoc :: {vis[this][n1]}
     vis[this][n1] ==> Set_ofSeq(lin)[n1]);
-  ensures {:layer 1} tableInv(table, abs, tabvis, lin, vis, tabLen, called, returned);
+  ensures {:layer 1} tableInv(table, abs, tabvis, hb, lin, vis, tabLen, called, returned);
   modifies returned;
 {
   yield;
-  assert {:layer 1} tableInv(table, abs, tabvis, lin, vis, tabLen, called, returned);
+  assert {:layer 1} tableInv(table, abs, tabvis, hb, lin, vis, tabLen, called, returned);
   assert {:layer 1} postLP(called, returned, lin, this);
   assert {:layer 1} (forall n1: Invoc :: {vis[this][n1]}
     vis[this][n1] ==> Set_ofSeq(lin)[n1]);
@@ -651,39 +676,39 @@ procedure {:yields} {:layer 1} {:refines "get_return_atomic"}
   call intro_writeReturned(this);
 
   yield;
-  assert {:layer 1} tableInv(table, abs, tabvis, lin, vis, tabLen, called, returned);
+  assert {:layer 1} tableInv(table, abs, tabvis, hb, lin, vis, tabLen, called, returned);
 }
 
 
 procedure {:yields} {:layer 1} {:refines "contains_call_atomic"}
     contains_call({:linear "this"} this: Invoc)
-  requires {:layer 1} tableInv(table, abs, tabvis, lin, vis, tabLen, called, returned);
+  requires {:layer 1} tableInv(table, abs, tabvis, hb, lin, vis, tabLen, called, returned);
   // everything before this has returned
-  requires {:layer 1} (forall n1: Invoc :: hb(n1, this) ==> returned[n1]);
+  requires {:layer 1} (forall n1: Invoc :: hb[n1][this] ==> returned[n1]);
   // this has not been called or returned yet
   requires {:layer 1} (!called[this] && !returned[this]);
-  ensures {:layer 1} tableInv(table, abs, tabvis, lin, vis, tabLen, called, returned);
+  ensures {:layer 1} tableInv(table, abs, tabvis, hb, lin, vis, tabLen, called, returned);
   ensures {:layer 1} preLP(called, returned, lin, this);
   modifies called;
 {
   yield;
-  assert {:layer 1} tableInv(table, abs, tabvis, lin, vis, tabLen, called, returned);
-  assert {:layer 1} (forall n1: Invoc :: hb(n1, this) ==> returned[n1]);
+  assert {:layer 1} tableInv(table, abs, tabvis, hb, lin, vis, tabLen, called, returned);
+  assert {:layer 1} (forall n1: Invoc :: hb[n1][this] ==> returned[n1]);
   assert {:layer 1} (!called[this] && !returned[this]);
 
   call intro_writeCalled(this);
   yield;
-  assert {:layer 1} tableInv(table, abs, tabvis, lin, vis, tabLen, called, returned);
+  assert {:layer 1} tableInv(table, abs, tabvis, hb, lin, vis, tabLen, called, returned);
   assert {:layer 1} preLP(called, returned, lin, this);
 }
 
 procedure {:yields} {:layer 1} {:refines "contains_spec"}
     contains(v: int, {:linear "this"} this: Invoc)
   returns (res: bool, witness_k: int)
-  requires {:layer 1} tableInv(table, abs, tabvis, lin, vis, tabLen, called, returned);
+  requires {:layer 1} tableInv(table, abs, tabvis, hb, lin, vis, tabLen, called, returned);
   requires {:layer 1} preLP(called, returned, lin, this);
   requires {:layer 1} invoc_m(this) == Map.contains && invoc_v(this) == v;
-  ensures {:layer 1} tableInv(table, abs, tabvis, lin, vis, tabLen, called, returned);
+  ensures {:layer 1} tableInv(table, abs, tabvis, hb, lin, vis, tabLen, called, returned);
   ensures {:layer 1} postLP(called, returned, lin, this);
   ensures {:layer 1} (forall n1: Invoc :: {vis[this][n1]}
     vis[this][n1] ==> Set_ofSeq(lin)[n1]);
@@ -691,13 +716,13 @@ procedure {:yields} {:layer 1} {:refines "contains_spec"}
   var k, tv: int;
   var {:layer 1} my_vis, my_vis1: SetInvoc;
   yield;
-  assert {:layer 1} tableInv(table, abs, tabvis, lin, vis, tabLen, called, returned) && preLP(called, returned, lin, this);
+  assert {:layer 1} tableInv(table, abs, tabvis, hb, lin, vis, tabLen, called, returned) && preLP(called, returned, lin, this);
 
   k := 0;
   call my_vis := intro_readLin();
   yield;
-  assert {:layer 1} tableInv(table, abs, tabvis, lin, vis, tabLen, called, returned) && preLP(called, returned, lin, this);
-  assert {:layer 1} (forall j: Invoc :: hb(j, this) ==> Set_subset(vis[j], my_vis));
+  assert {:layer 1} tableInv(table, abs, tabvis, hb, lin, vis, tabLen, called, returned) && preLP(called, returned, lin, this);
+  assert {:layer 1} (forall j: Invoc :: hb[j][this] ==> Set_subset(vis[j], my_vis));
   assert {:layer 1} (forall n1: Invoc :: {my_vis[n1]}
     my_vis[n1] ==> Set_ofSeq(lin)[n1]);
   assert {:layer 1} (forall i: int :: 0 <= i && i < tabLen
@@ -705,10 +730,10 @@ procedure {:yields} {:layer 1} {:refines "contains_spec"}
 
   while (k < tabLen)
     invariant {:layer 1} 0 <= k && k <= tabLen;
-    invariant {:layer 1} tableInv(table, abs, tabvis, lin, vis, tabLen, called, returned) && preLP(called, returned, lin, this);
+    invariant {:layer 1} tableInv(table, abs, tabvis, hb, lin, vis, tabLen, called, returned) && preLP(called, returned, lin, this);
     invariant {:layer 1} (forall i: int :: 0 <= i && i < k
       ==> Map.ofSeq(Seq_restr(lin, my_vis))[i] != v);
-    invariant {:layer 1} (forall j: Invoc :: hb(j, this) ==> Set_subset(vis[j], my_vis));
+    invariant {:layer 1} (forall j: Invoc :: hb[j][this] ==> Set_subset(vis[j], my_vis));
     invariant {:layer 1} (forall n1: Invoc :: {my_vis[n1]}
       my_vis[n1] ==> Set_ofSeq(lin)[n1]);
     invariant {:layer 1} (forall i: int :: 0 <= i && i < tabLen
@@ -735,7 +760,7 @@ procedure {:yields} {:layer 1} {:refines "contains_spec"}
 
       res := true;
 
-      yield; assert {:layer 1} tableInv(table, abs, tabvis, lin, vis, tabLen, called, returned)
+      yield; assert {:layer 1} tableInv(table, abs, tabvis, hb, lin, vis, tabLen, called, returned)
         && postLP(called, returned, lin, this);
       assert {:layer 1} (forall n1: Invoc :: {vis[this][n1]}
         vis[this][n1] ==> Set_ofSeq(lin)[n1]);
@@ -743,20 +768,20 @@ procedure {:yields} {:layer 1} {:refines "contains_spec"}
     }
     k := k + 1;
     yield;
-    assert {:layer 1} tableInv(table, abs, tabvis, lin, vis, tabLen, called, returned) && preLP(called, returned, lin, this);
+    assert {:layer 1} tableInv(table, abs, tabvis, hb, lin, vis, tabLen, called, returned) && preLP(called, returned, lin, this);
     assert {:layer 1} (forall i: int :: 0 <= i && i < k
       ==> Map.ofSeq(Seq_restr(lin, my_vis))[i] != v);
-    assert {:layer 1} (forall j: Invoc :: hb(j, this) ==> Set_subset(vis[j], my_vis));
+    assert {:layer 1} (forall j: Invoc :: hb[j][this] ==> Set_subset(vis[j], my_vis));
     assert {:layer 1} (forall n1: Invoc :: {my_vis[n1]}
       my_vis[n1] ==> Set_ofSeq(lin)[n1]);
     assert {:layer 1} (forall i: int :: 0 <= i && i < tabLen
       ==> Set_subset(Map.restr(my_vis, i), tabvis[i]));
   }
   yield;
-  assert {:layer 1} tableInv(table, abs, tabvis, lin, vis, tabLen, called, returned) && preLP(called, returned, lin, this);
+  assert {:layer 1} tableInv(table, abs, tabvis, hb, lin, vis, tabLen, called, returned) && preLP(called, returned, lin, this);
   assert {:layer 1} (forall i: int :: 0 <= i && i < tabLen
     ==> Map.ofSeq(Seq_restr(lin, my_vis))[i] != v);
-  assert {:layer 1} (forall j: Invoc :: hb(j, this) ==> Set_subset(vis[j], my_vis));
+  assert {:layer 1} (forall j: Invoc :: hb[j][this] ==> Set_subset(vis[j], my_vis));
   assert {:layer 1} (forall n1: Invoc :: {my_vis[n1]}
     my_vis[n1] ==> Set_ofSeq(lin)[n1]);
 
@@ -767,7 +792,7 @@ procedure {:yields} {:layer 1} {:refines "contains_spec"}
 
   res := false;
 
-  yield; assert {:layer 1} tableInv(table, abs, tabvis, lin, vis, tabLen, called, returned)
+  yield; assert {:layer 1} tableInv(table, abs, tabvis, hb, lin, vis, tabLen, called, returned)
     && postLP(called, returned, lin, this);
   assert {:layer 1} (forall n1: Invoc :: {vis[this][n1]}
     vis[this][n1] ==> Set_ofSeq(lin)[n1]);
@@ -775,15 +800,15 @@ procedure {:yields} {:layer 1} {:refines "contains_spec"}
 
 procedure {:yields} {:layer 1} {:refines "contains_return_atomic"}
     contains_return({:linear "this"} this: Invoc)
-  requires {:layer 1} tableInv(table, abs, tabvis, lin, vis, tabLen, called, returned);
+  requires {:layer 1} tableInv(table, abs, tabvis, hb, lin, vis, tabLen, called, returned);
   requires {:layer 1} postLP(called, returned, lin, this);
   requires {:layer 1} (forall n1: Invoc :: {vis[this][n1]}
     vis[this][n1] ==> Set_ofSeq(lin)[n1]);
-  ensures {:layer 1} tableInv(table, abs, tabvis, lin, vis, tabLen, called, returned);
+  ensures {:layer 1} tableInv(table, abs, tabvis, hb, lin, vis, tabLen, called, returned);
   modifies returned;
 {
   yield;
-  assert {:layer 1} tableInv(table, abs, tabvis, lin, vis, tabLen, called, returned);
+  assert {:layer 1} tableInv(table, abs, tabvis, hb, lin, vis, tabLen, called, returned);
   assert {:layer 1} postLP(called, returned, lin, this);
   assert {:layer 1} (forall n1: Invoc :: {vis[this][n1]}
     vis[this][n1] ==> Set_ofSeq(lin)[n1]);
@@ -791,5 +816,5 @@ procedure {:yields} {:layer 1} {:refines "contains_return_atomic"}
   call intro_writeReturned(this);
 
   yield;
-  assert {:layer 1} tableInv(table, abs, tabvis, lin, vis, tabLen, called, returned);
+  assert {:layer 1} tableInv(table, abs, tabvis, hb, lin, vis, tabLen, called, returned);
 }
