proofs/impls/ms-queue.bpl
@@ -55,7 +55,7 @@ var {:layer 1,1} absRefs: [int]Ref;  // connection between abstract and concrete
 function {:inline} Inv(queueFP: [Ref]bool, usedFP: [Ref]bool, start: Ref,
     head: Ref, tail: Ref, next: [Ref]Ref, data: [Ref]Key,
     nextTags: [Ref]SetInvoc, nextInvoc: [Ref]Invoc, nextRef: [Invoc]Ref,
-    lin: SeqInvoc, vis: [Invoc]SetInvoc, absRefs: [int]Ref,
+    hb: [Invoc][Invoc]bool, lin: SeqInvoc, vis: [Invoc]SetInvoc, absRefs: [int]Ref,
     called: [Invoc]bool, returned: [Invoc]bool) : bool
 {
   // There is a list from head to null
@@ -92,7 +92,7 @@ function {:inline} Inv(queueFP: [Ref]bool, usedFP: [Ref]bool, start: Ref,
   && nextTags[absRefs[Queue.stateTail(Queue.ofSeq(lin)) - 1]] == Set_empty()
   // lin is made up of nextInvoc[y] for y in the queue
   && (forall n: Invoc :: {Seq_elem(n, lin)} known(nextRef[n]) && invoc_m(n) == Queue.push ==>
-    (Seq_elem(n, lin) 
+    (Seq_elem(n, lin)
       <==> Btwn(next, start, nextRef[n], null)
         && nextRef[n] != null && next[nextRef[n]] != null))
   // lin is ordered by order of nodes in queue
@@ -122,7 +122,7 @@ function {:inline} Inv(queueFP: [Ref]bool, usedFP: [Ref]bool, start: Ref,
   && (forall n1, n2: Invoc :: {vis[n2][n1]}
   vis[n2][n1] && returned[n2] ==> Set_ofSeq(lin)[n1])
   // Used to infer that invocations don't modify vis after they've returned
-  && (forall n1, n2 : Invoc :: called[n1] && hb(n2, n1) ==> returned[n2])
+  && (forall n1, n2 : Invoc :: called[n1] && hb[n2][n1] ==> returned[n2])
   // To establish precondition of intro_writeLin
   && (forall n: Invoc :: returned[n] ==> Seq_elem(n, lin))
   // Axiom of heap encoding
@@ -275,7 +275,7 @@ procedure {:layer 1} {:inline 1} intro_writeNextInvoc(x: Ref, n: Invoc)
 }
 
 procedure {:layer 1} intro_readNextTags(x: Ref, v: SetInvoc) returns (v1: SetInvoc)
-  requires {:layer 1} Inv(queueFP, usedFP, start, head, tail, next, data, nextTags, nextInvoc, nextRef, lin, vis, absRefs, called, returned);
+  requires {:layer 1} Inv(queueFP, usedFP, start, head, tail, next, data, nextTags, nextInvoc, nextRef, hb, lin, vis, absRefs, called, returned);
   requires {:layer 1} known(x) && Btwn(next, start, x, null) && x != null;
   ensures {:layer 1} next[x] == null ==> v1 == v;
   ensures {:layer 1} next[x] != null ==> Seq_elem(nextInvoc[x], lin) && v1 == Set_add(v, nextInvoc[x]);
@@ -303,33 +303,42 @@ procedure {:layer 1} {:inline 1} intro_writeReturned({:linear "this"} this: Invo
 // ---------- Implementation of Queue:
 
 
+procedure {:yields} {:layer 1} {:refines "hb_action_atomic"}
+    hb_action(n1: Invoc, n2: Invoc)
+  requires {:layer 1} returned[n1] && !called[n2];
+{
+  call intro_writeHb(n1, n2);
+  yield;
+}
+
+
 procedure {:yields} {:layer 1} {:refines "pop_call_atomic"}
     pop_call({:linear "this"} this: Invoc)
-  requires {:layer 1} Inv(queueFP, usedFP, start, head, tail, next, data, nextTags, nextInvoc, nextRef, lin, vis, absRefs, called, returned);
+  requires {:layer 1} Inv(queueFP, usedFP, start, head, tail, next, data, nextTags, nextInvoc, nextRef, hb, lin, vis, absRefs, called, returned);
   // everything before this has returned
-  requires {:layer 1} (forall n1: Invoc :: hb(n1, this) ==> returned[n1]);
+  requires {:layer 1} (forall n1: Invoc :: hb[n1][this] ==> returned[n1]);
   // this has not been called or returned yet
   requires {:layer 1} (!called[this] && !returned[this]);
-  ensures {:layer 1} Inv(queueFP, usedFP, start, head, tail, next, data, nextTags, nextInvoc, nextRef, lin, vis, absRefs, called, returned);
+  ensures {:layer 1} Inv(queueFP, usedFP, start, head, tail, next, data, nextTags, nextInvoc, nextRef, hb, lin, vis, absRefs, called, returned);
   ensures {:layer 1} preLP(called, returned, lin, this);
   modifies called;
 {
   yield;
-  assert {:layer 1} Inv(queueFP, usedFP, start, head, tail, next, data, nextTags, nextInvoc, nextRef, lin, vis, absRefs, called, returned);
-  assert {:layer 1} (forall n1: Invoc :: hb(n1, this) ==> returned[n1]);
+  assert {:layer 1} Inv(queueFP, usedFP, start, head, tail, next, data, nextTags, nextInvoc, nextRef, hb, lin, vis, absRefs, called, returned);
+  assert {:layer 1} (forall n1: Invoc :: hb[n1][this] ==> returned[n1]);
   assert {:layer 1} (!called[this] && !returned[this]);
 
   call intro_writeCalled(this);
   yield;
-  assert {:layer 1} Inv(queueFP, usedFP, start, head, tail, next, data, nextTags, nextInvoc, nextRef, lin, vis, absRefs, called, returned);
+  assert {:layer 1} Inv(queueFP, usedFP, start, head, tail, next, data, nextTags, nextInvoc, nextRef, hb, lin, vis, absRefs, called, returned);
   assert {:layer 1} preLP(called, returned, lin, this);
 }
 
 procedure {:yields} {:layer 1} {:refines "pop_atomic"} pop({:linear "this"} this: Invoc)
   returns (k: Key)
-  requires {:layer 1} Inv(queueFP, usedFP, start, head, tail, next, data, nextTags, nextInvoc, nextRef, lin, vis, absRefs, called, returned) && preLP(called, returned, lin, this);
+  requires {:layer 1} Inv(queueFP, usedFP, start, head, tail, next, data, nextTags, nextInvoc, nextRef, hb, lin, vis, absRefs, called, returned) && preLP(called, returned, lin, this);
   requires {:layer 1} invoc_m(this) == Queue.pop;
-  ensures {:layer 1} Inv(queueFP, usedFP, start, head, tail, next, data, nextTags, nextInvoc, nextRef, lin, vis, absRefs, called, returned) && postLP(called, returned, lin, this);
+  ensures {:layer 1} Inv(queueFP, usedFP, start, head, tail, next, data, nextTags, nextInvoc, nextRef, hb, lin, vis, absRefs, called, returned) && postLP(called, returned, lin, this);
   ensures {:layer 1} (forall n1: Invoc :: {vis[this][n1]}
     vis[this][n1] ==> Set_ofSeq(lin)[n1]);
 {
@@ -338,27 +347,27 @@ procedure {:yields} {:layer 1} {:refines "pop_atomic"} pop({:linear "this"} this
   var h, t, hn: Ref;
 
   yield;
-  assert {:layer 1} Inv(queueFP, usedFP, start, head, tail, next, data, nextTags, nextInvoc, nextRef, lin, vis, absRefs, called, returned) && preLP(called, returned, lin, this);
+  assert {:layer 1} Inv(queueFP, usedFP, start, head, tail, next, data, nextTags, nextInvoc, nextRef, hb, lin, vis, absRefs, called, returned) && preLP(called, returned, lin, this);
 
   yield;
-  assert {:layer 1} Inv(queueFP, usedFP, start, head, tail, next, data, nextTags, nextInvoc, nextRef, lin, vis, absRefs, called, returned) && preLP(called, returned, lin, this);
+  assert {:layer 1} Inv(queueFP, usedFP, start, head, tail, next, data, nextTags, nextInvoc, nextRef, hb, lin, vis, absRefs, called, returned) && preLP(called, returned, lin, this);
   while (true)
-    invariant {:layer 1} Inv(queueFP, usedFP, start, head, tail, next, data, nextTags, nextInvoc, nextRef, lin, vis, absRefs, called, returned) && preLP(called, returned, lin, this);
+    invariant {:layer 1} Inv(queueFP, usedFP, start, head, tail, next, data, nextTags, nextInvoc, nextRef, hb, lin, vis, absRefs, called, returned) && preLP(called, returned, lin, this);
   {
     call h := readHead();
     yield;
-    assert {:layer 1} Inv(queueFP, usedFP, start, head, tail, next, data, nextTags, nextInvoc, nextRef, lin, vis, absRefs, called, returned) && preLP(called, returned, lin, this);
+    assert {:layer 1} Inv(queueFP, usedFP, start, head, tail, next, data, nextTags, nextInvoc, nextRef, hb, lin, vis, absRefs, called, returned) && preLP(called, returned, lin, this);
     assert {:layer 1} h == head || usedFP[h];
 
     call t := readTail();
     yield;
-    assert {:layer 1} Inv(queueFP, usedFP, start, head, tail, next, data, nextTags, nextInvoc, nextRef, lin, vis, absRefs, called, returned) && preLP(called, returned, lin, this);
+    assert {:layer 1} Inv(queueFP, usedFP, start, head, tail, next, data, nextTags, nextInvoc, nextRef, hb, lin, vis, absRefs, called, returned) && preLP(called, returned, lin, this);
     assert {:layer 1} h == head || usedFP[h];
     assert {:layer 1} (h == head && h != t ==> head != tail);
 
     call hn := readNext(h);
     yield;
-    assert {:layer 1} Inv(queueFP, usedFP, start, head, tail, next, data, nextTags, nextInvoc, nextRef, lin, vis, absRefs, called, returned) && preLP(called, returned, lin, this);
+    assert {:layer 1} Inv(queueFP, usedFP, start, head, tail, next, data, nextTags, nextInvoc, nextRef, hb, lin, vis, absRefs, called, returned) && preLP(called, returned, lin, this);
     assert {:layer 1} h == head || usedFP[h];
     assert {:layer 1} (h == t && hn == null) || queueFP[hn] || usedFP[hn];
     assert {:layer 1} (h == head && h != t ==> head != tail && hn == next[head]);
@@ -366,7 +375,7 @@ procedure {:yields} {:layer 1} {:refines "pop_atomic"} pop({:linear "this"} this
     if (h != t) {
       call k := readData(hn);
       yield;
-      assert {:layer 1} Inv(queueFP, usedFP, start, head, tail, next, data, nextTags, nextInvoc, nextRef, lin, vis, absRefs, called, returned) && preLP(called, returned, lin, this);
+      assert {:layer 1} Inv(queueFP, usedFP, start, head, tail, next, data, nextTags, nextInvoc, nextRef, hb, lin, vis, absRefs, called, returned) && preLP(called, returned, lin, this);
       assert {:layer 1} h == head || usedFP[h];
       assert {:layer 1} (h == head && h != t ==> head != tail && hn == next[head]);
       assert {:layer 1} data[hn] == k;
@@ -382,25 +391,25 @@ procedure {:yields} {:layer 1} {:refines "pop_atomic"} pop({:linear "this"} this
       }
     }
     yield;
-    assert {:layer 1} Inv(queueFP, usedFP, start, head, tail, next, data, nextTags, nextInvoc, nextRef, lin, vis, absRefs, called, returned) && preLP(called, returned, lin, this);
+    assert {:layer 1} Inv(queueFP, usedFP, start, head, tail, next, data, nextTags, nextInvoc, nextRef, hb, lin, vis, absRefs, called, returned) && preLP(called, returned, lin, this);
   }
   yield;
-  assert {:layer 1} Inv(queueFP, usedFP, start, head, tail, next, data, nextTags, nextInvoc, nextRef, lin, vis, absRefs, called, returned) && postLP(called, returned, lin, this);
+  assert {:layer 1} Inv(queueFP, usedFP, start, head, tail, next, data, nextTags, nextInvoc, nextRef, hb, lin, vis, absRefs, called, returned) && postLP(called, returned, lin, this);
   assert {:layer 1} (forall n1: Invoc :: {vis[this][n1]}
     vis[this][n1] ==> Set_ofSeq(lin)[n1]);
 }
 
 procedure {:yields} {:layer 1} {:refines "pop_return_atomic"}
     pop_return({:linear "this"} this: Invoc)
-  requires {:layer 1} Inv(queueFP, usedFP, start, head, tail, next, data, nextTags, nextInvoc, nextRef, lin, vis, absRefs, called, returned);
+  requires {:layer 1} Inv(queueFP, usedFP, start, head, tail, next, data, nextTags, nextInvoc, nextRef, hb, lin, vis, absRefs, called, returned);
   requires {:layer 1} postLP(called, returned, lin, this);
   requires {:layer 1} (forall n1: Invoc :: {vis[this][n1]}
     vis[this][n1] ==> Set_ofSeq(lin)[n1]);
-  ensures {:layer 1} Inv(queueFP, usedFP, start, head, tail, next, data, nextTags, nextInvoc, nextRef, lin, vis, absRefs, called, returned);
+  ensures {:layer 1} Inv(queueFP, usedFP, start, head, tail, next, data, nextTags, nextInvoc, nextRef, hb, lin, vis, absRefs, called, returned);
   modifies returned;
 {
   yield;
-  assert {:layer 1} Inv(queueFP, usedFP, start, head, tail, next, data, nextTags, nextInvoc, nextRef, lin, vis, absRefs, called, returned);
+  assert {:layer 1} Inv(queueFP, usedFP, start, head, tail, next, data, nextTags, nextInvoc, nextRef, hb, lin, vis, absRefs, called, returned);
   assert {:layer 1} postLP(called, returned, lin, this);
   assert {:layer 1} (forall n1: Invoc :: {vis[this][n1]}
     vis[this][n1] ==> Set_ofSeq(lin)[n1]);
@@ -408,29 +417,29 @@ procedure {:yields} {:layer 1} {:refines "pop_return_atomic"}
   call intro_writeReturned(this);
 
   yield;
-  assert {:layer 1} Inv(queueFP, usedFP, start, head, tail, next, data, nextTags, nextInvoc, nextRef, lin, vis, absRefs, called, returned);
+  assert {:layer 1} Inv(queueFP, usedFP, start, head, tail, next, data, nextTags, nextInvoc, nextRef, hb, lin, vis, absRefs, called, returned);
 }
 
 
 procedure {:yields} {:layer 1} {:refines "push_call_atomic"}
     push_call({:linear "this"} this: Invoc)
-  requires {:layer 1} Inv(queueFP, usedFP, start, head, tail, next, data, nextTags, nextInvoc, nextRef, lin, vis, absRefs, called, returned);
+  requires {:layer 1} Inv(queueFP, usedFP, start, head, tail, next, data, nextTags, nextInvoc, nextRef, hb, lin, vis, absRefs, called, returned);
   // everything before this has returned
-  requires {:layer 1} (forall n1: Invoc :: hb(n1, this) ==> returned[n1]);
+  requires {:layer 1} (forall n1: Invoc :: hb[n1][this] ==> returned[n1]);
   // this has not been called or returned yet
   requires {:layer 1} (!called[this] && !returned[this]);
-  ensures {:layer 1} Inv(queueFP, usedFP, start, head, tail, next, data, nextTags, nextInvoc, nextRef, lin, vis, absRefs, called, returned);
+  ensures {:layer 1} Inv(queueFP, usedFP, start, head, tail, next, data, nextTags, nextInvoc, nextRef, hb, lin, vis, absRefs, called, returned);
   ensures {:layer 1} preLP(called, returned, lin, this);
   modifies called;
 {
   yield;
-  assert {:layer 1} Inv(queueFP, usedFP, start, head, tail, next, data, nextTags, nextInvoc, nextRef, lin, vis, absRefs, called, returned);
-  assert {:layer 1} (forall n1: Invoc :: hb(n1, this) ==> returned[n1]);
+  assert {:layer 1} Inv(queueFP, usedFP, start, head, tail, next, data, nextTags, nextInvoc, nextRef, hb, lin, vis, absRefs, called, returned);
+  assert {:layer 1} (forall n1: Invoc :: hb[n1][this] ==> returned[n1]);
   assert {:layer 1} (!called[this] && !returned[this]);
 
   call intro_writeCalled(this);
   yield;
-  assert {:layer 1} Inv(queueFP, usedFP, start, head, tail, next, data, nextTags, nextInvoc, nextRef, lin, vis, absRefs, called, returned);
+  assert {:layer 1} Inv(queueFP, usedFP, start, head, tail, next, data, nextTags, nextInvoc, nextRef, hb, lin, vis, absRefs, called, returned);
   assert {:layer 1} preLP(called, returned, lin, this);
 }
 
@@ -438,9 +447,9 @@ procedure {:yields} {:layer 1} {:refines "push_atomic"} push(k: Key, x: Ref,
     {:linear_in "FP"} xFP: [Ref]bool, {:linear "this"} this: Invoc)
   requires {:layer 1} xFP[x] && next[x] == null && data[x] == k && nextTags[x] == Set_empty();
   requires {:layer 1} !Btwn(next, head, x, null);
-  requires {:layer 1} Inv(queueFP, usedFP, start, head, tail, next, data, nextTags, nextInvoc, nextRef, lin, vis, absRefs, called, returned) && preLP(called, returned, lin, this);
+  requires {:layer 1} Inv(queueFP, usedFP, start, head, tail, next, data, nextTags, nextInvoc, nextRef, hb, lin, vis, absRefs, called, returned) && preLP(called, returned, lin, this);
   requires {:layer 1} invoc_m(this) == Queue.push && invoc_k(this) == k;
-  ensures {:layer 1} Inv(queueFP, usedFP, start, head, tail, next, data, nextTags, nextInvoc, nextRef, lin, vis, absRefs, called, returned) && postLP(called, returned, lin, this);
+  ensures {:layer 1} Inv(queueFP, usedFP, start, head, tail, next, data, nextTags, nextInvoc, nextRef, hb, lin, vis, absRefs, called, returned) && postLP(called, returned, lin, this);
 {
   var {:layer 1} my_vis: SetInvoc;
   var t, tn: Ref;
@@ -448,18 +457,18 @@ procedure {:yields} {:layer 1} {:refines "push_atomic"} push(k: Key, x: Ref,
   var {:linear "FP"} tFP: [Ref]bool;
 
   yield;
-  assert {:layer 1} Inv(queueFP, usedFP, start, head, tail, next, data, nextTags, nextInvoc, nextRef, lin, vis, absRefs, called, returned) && preLP(called, returned, lin, this);
+  assert {:layer 1} Inv(queueFP, usedFP, start, head, tail, next, data, nextTags, nextInvoc, nextRef, hb, lin, vis, absRefs, called, returned) && preLP(called, returned, lin, this);
   assert {:layer 1} !Btwn(next, head, x, null);
   assert {:layer 1} xFP[x] && next[x] == null && data[x] == k && nextTags[x] == Set_empty();
   tFP := xFP;
   while (true)
-    invariant {:layer 1} Inv(queueFP, usedFP, start, head, tail, next, data, nextTags, nextInvoc, nextRef, lin, vis, absRefs, called, returned) && preLP(called, returned, lin, this);
+    invariant {:layer 1} Inv(queueFP, usedFP, start, head, tail, next, data, nextTags, nextInvoc, nextRef, hb, lin, vis, absRefs, called, returned) && preLP(called, returned, lin, this);
     invariant {:layer 1} known(x) && !Btwn(next, head, x, null);
     invariant {:layer 1} tFP == xFP && xFP[x] && next[x] == null && data[x] == k && nextTags[x] == Set_empty();
   {
     call t := readTail();
     yield;
-    assert {:layer 1} Inv(queueFP, usedFP, start, head, tail, next, data, nextTags, nextInvoc, nextRef, lin, vis, absRefs, called, returned) && preLP(called, returned, lin, this);
+    assert {:layer 1} Inv(queueFP, usedFP, start, head, tail, next, data, nextTags, nextInvoc, nextRef, hb, lin, vis, absRefs, called, returned) && preLP(called, returned, lin, this);
     assert {:layer 1} !Btwn(next, head, x, null);
     assert {:layer 1} tFP == xFP && xFP[x] && next[x] == null && data[x] == k && nextTags[x] == Set_empty();
     assert {:layer 1} t != null && (queueFP[t] || usedFP[t]);
@@ -467,7 +476,7 @@ procedure {:yields} {:layer 1} {:refines "push_atomic"} push(k: Key, x: Ref,
 
     call tn := readNext(t);
     yield;
-    assert {:layer 1} Inv(queueFP, usedFP, start, head, tail, next, data, nextTags, nextInvoc, nextRef, lin, vis, absRefs, called, returned) && preLP(called, returned, lin, this);
+    assert {:layer 1} Inv(queueFP, usedFP, start, head, tail, next, data, nextTags, nextInvoc, nextRef, hb, lin, vis, absRefs, called, returned) && preLP(called, returned, lin, this);
     assert {:layer 1} !Btwn(next, head, x, null);
     assert {:layer 1} tFP == xFP && xFP[x] && next[x] == null && data[x] == k && nextTags[x] == Set_empty();
     assert {:layer 1} t != null && (queueFP[t] || usedFP[t]);
@@ -490,27 +499,27 @@ procedure {:yields} {:layer 1} {:refines "push_atomic"} push(k: Key, x: Ref,
       call b := casTail(t, tn, this);
     }
     yield;
-    assert {:layer 1} Inv(queueFP, usedFP, start, head, tail, next, data, nextTags, nextInvoc, nextRef, lin, vis, absRefs, called, returned) && preLP(called, returned, lin, this);
+    assert {:layer 1} Inv(queueFP, usedFP, start, head, tail, next, data, nextTags, nextInvoc, nextRef, hb, lin, vis, absRefs, called, returned) && preLP(called, returned, lin, this);
     assert {:layer 1} !Btwn(next, head, x, null);
     assert {:layer 1} tFP == xFP && xFP[x] && next[x] == null && data[x] == k && nextTags[x] == Set_empty();
   }
   yield;
-  assert {:layer 1} Inv(queueFP, usedFP, start, head, tail, next, data, nextTags, nextInvoc, nextRef, lin, vis, absRefs, called, returned) && postLP(called, returned, lin, this);
+  assert {:layer 1} Inv(queueFP, usedFP, start, head, tail, next, data, nextTags, nextInvoc, nextRef, hb, lin, vis, absRefs, called, returned) && postLP(called, returned, lin, this);
   assert {:layer 1} (forall n1: Invoc :: {vis[this][n1]}
     vis[this][n1] ==> Set_ofSeq(lin)[n1]);
 }
 
 procedure {:yields} {:layer 1} {:refines "push_return_atomic"}
     push_return({:linear "this"} this: Invoc)
-  requires {:layer 1} Inv(queueFP, usedFP, start, head, tail, next, data, nextTags, nextInvoc, nextRef, lin, vis, absRefs, called, returned);
+  requires {:layer 1} Inv(queueFP, usedFP, start, head, tail, next, data, nextTags, nextInvoc, nextRef, hb, lin, vis, absRefs, called, returned);
   requires {:layer 1} postLP(called, returned, lin, this);
   requires {:layer 1} (forall n1: Invoc :: {vis[this][n1]}
     vis[this][n1] ==> Set_ofSeq(lin)[n1]);
-  ensures {:layer 1} Inv(queueFP, usedFP, start, head, tail, next, data, nextTags, nextInvoc, nextRef, lin, vis, absRefs, called, returned);
+  ensures {:layer 1} Inv(queueFP, usedFP, start, head, tail, next, data, nextTags, nextInvoc, nextRef, hb, lin, vis, absRefs, called, returned);
   modifies returned;
 {
   yield;
-  assert {:layer 1} Inv(queueFP, usedFP, start, head, tail, next, data, nextTags, nextInvoc, nextRef, lin, vis, absRefs, called, returned);
+  assert {:layer 1} Inv(queueFP, usedFP, start, head, tail, next, data, nextTags, nextInvoc, nextRef, hb, lin, vis, absRefs, called, returned);
   assert {:layer 1} postLP(called, returned, lin, this);
   assert {:layer 1} (forall n1: Invoc :: {vis[this][n1]}
     vis[this][n1] ==> Set_ofSeq(lin)[n1]);
@@ -518,36 +527,36 @@ procedure {:yields} {:layer 1} {:refines "push_return_atomic"}
   call intro_writeReturned(this);
 
   yield;
-  assert {:layer 1} Inv(queueFP, usedFP, start, head, tail, next, data, nextTags, nextInvoc, nextRef, lin, vis, absRefs, called, returned);
+  assert {:layer 1} Inv(queueFP, usedFP, start, head, tail, next, data, nextTags, nextInvoc, nextRef, hb, lin, vis, absRefs, called, returned);
 }
 
 
 procedure {:yields} {:layer 1} {:refines "size_call_atomic"}
     size_call({:linear "this"} this: Invoc)
-  requires {:layer 1} Inv(queueFP, usedFP, start, head, tail, next, data, nextTags, nextInvoc, nextRef, lin, vis, absRefs, called, returned);
+  requires {:layer 1} Inv(queueFP, usedFP, start, head, tail, next, data, nextTags, nextInvoc, nextRef, hb, lin, vis, absRefs, called, returned);
   // everything before this has returned
-  requires {:layer 1} (forall n1: Invoc :: hb(n1, this) ==> returned[n1]);
+  requires {:layer 1} (forall n1: Invoc :: hb[n1][this] ==> returned[n1]);
   // this has not been called or returned yet
   requires {:layer 1} (!called[this] && !returned[this]);
-  ensures {:layer 1} Inv(queueFP, usedFP, start, head, tail, next, data, nextTags, nextInvoc, nextRef, lin, vis, absRefs, called, returned);
+  ensures {:layer 1} Inv(queueFP, usedFP, start, head, tail, next, data, nextTags, nextInvoc, nextRef, hb, lin, vis, absRefs, called, returned);
   ensures {:layer 1} preLP(called, returned, lin, this);
   modifies called;
 {
   yield;
-  assert {:layer 1} Inv(queueFP, usedFP, start, head, tail, next, data, nextTags, nextInvoc, nextRef, lin, vis, absRefs, called, returned);
-  assert {:layer 1} (forall n1: Invoc :: hb(n1, this) ==> returned[n1]);
+  assert {:layer 1} Inv(queueFP, usedFP, start, head, tail, next, data, nextTags, nextInvoc, nextRef, hb, lin, vis, absRefs, called, returned);
+  assert {:layer 1} (forall n1: Invoc :: hb[n1][this] ==> returned[n1]);
   assert {:layer 1} (!called[this] && !returned[this]);
 
   call intro_writeCalled(this);
   yield;
-  assert {:layer 1} Inv(queueFP, usedFP, start, head, tail, next, data, nextTags, nextInvoc, nextRef, lin, vis, absRefs, called, returned);
+  assert {:layer 1} Inv(queueFP, usedFP, start, head, tail, next, data, nextTags, nextInvoc, nextRef, hb, lin, vis, absRefs, called, returned);
   assert {:layer 1} preLP(called, returned, lin, this);
 }
 
 procedure {:yields} {:layer 1} {:refines "size_atomic"} size({:linear "this"} this: Invoc) returns (s: int)
-  requires {:layer 1} Inv(queueFP, usedFP, start, head, tail, next, data, nextTags, nextInvoc, nextRef, lin, vis, absRefs, called, returned) && preLP(called, returned, lin, this);
+  requires {:layer 1} Inv(queueFP, usedFP, start, head, tail, next, data, nextTags, nextInvoc, nextRef, hb, lin, vis, absRefs, called, returned) && preLP(called, returned, lin, this);
   requires {:layer 1} invoc_m(this) == Queue.size;
-  ensures {:layer 1} Inv(queueFP, usedFP, start, head, tail, next, data, nextTags, nextInvoc, nextRef, lin, vis, absRefs, called, returned) && postLP(called, returned, lin, this);
+  ensures {:layer 1} Inv(queueFP, usedFP, start, head, tail, next, data, nextTags, nextInvoc, nextRef, hb, lin, vis, absRefs, called, returned) && postLP(called, returned, lin, this);
 {
   var {:layer 1} my_vis: SetInvoc;
   var {:layer 1} t0i: int; var {:layer 1} ci: int;
@@ -557,7 +566,7 @@ procedure {:yields} {:layer 1} {:refines "size_atomic"} size({:linear "this"} th
   var {:layer 1} old_c: Ref;
 
   yield;
-  assert {:layer 1} Inv(queueFP, usedFP, start, head, tail, next, data, nextTags, nextInvoc, nextRef, lin, vis, absRefs, called, returned) && preLP(called, returned, lin, this);
+  assert {:layer 1} Inv(queueFP, usedFP, start, head, tail, next, data, nextTags, nextInvoc, nextRef, hb, lin, vis, absRefs, called, returned) && preLP(called, returned, lin, this);
 
   s := 0;
   call c := readHead();
@@ -567,8 +576,8 @@ procedure {:yields} {:layer 1} {:refines "size_atomic"} size({:linear "this"} th
   call my_vis := intro_readLin();
 
   yield;
-  assert {:layer 1} Inv(queueFP, usedFP, start, head, tail, next, data, nextTags, nextInvoc, nextRef, lin, vis, absRefs, called, returned) && preLP(called, returned, lin, this);
-  assert {:layer 1} (forall j: Invoc :: hb(j, this) ==> Set_subset(vis[j], my_vis));
+  assert {:layer 1} Inv(queueFP, usedFP, start, head, tail, next, data, nextTags, nextInvoc, nextRef, hb, lin, vis, absRefs, called, returned) && preLP(called, returned, lin, this);
+  assert {:layer 1} (forall j: Invoc :: hb[j][this] ==> Set_subset(vis[j], my_vis));
   assert {:layer 1} (forall n1: Invoc :: {my_vis[n1]}
     my_vis[n1] ==> Set_ofSeq(lin)[n1]);
   assert {:layer 1} (usedFP[c] || queueFP[c]);
@@ -607,8 +616,8 @@ procedure {:yields} {:layer 1} {:refines "size_atomic"} size({:linear "this"} th
       && s == ci - 1 - Queue.stateHead(Queue.ofSeq(Seq_restr(lin, my_vis)));
 
   yield;
-  assert {:layer 1} Inv(queueFP, usedFP, start, head, tail, next, data, nextTags, nextInvoc, nextRef, lin, vis, absRefs, called, returned) && preLP(called, returned, lin, this);
-  assert {:layer 1} (forall j: Invoc :: hb(j, this) ==> Set_subset(vis[j], my_vis));
+  assert {:layer 1} Inv(queueFP, usedFP, start, head, tail, next, data, nextTags, nextInvoc, nextRef, hb, lin, vis, absRefs, called, returned) && preLP(called, returned, lin, this);
+  assert {:layer 1} (forall j: Invoc :: hb[j][this] ==> Set_subset(vis[j], my_vis));
   assert {:layer 1} (forall n1: Invoc :: {my_vis[n1]}
     my_vis[n1] ==> Set_ofSeq(lin)[n1]);
   assert {:layer 1} (usedFP[c] || queueFP[c]) && known(c) && (cn != null ==> cn == next[c]);
@@ -633,9 +642,9 @@ procedure {:yields} {:layer 1} {:refines "size_atomic"} size({:linear "this"} th
     && invoc_m(n2) == Queue.push ==> Seq_ord(lin, n1, n2)));
 
   while (cn != null)
-    invariant {:layer 1} Inv(queueFP, usedFP, start, head, tail, next, data, nextTags, nextInvoc, nextRef, lin, vis, absRefs, called, returned) && preLP(called, returned, lin, this);
+    invariant {:layer 1} Inv(queueFP, usedFP, start, head, tail, next, data, nextTags, nextInvoc, nextRef, hb, lin, vis, absRefs, called, returned) && preLP(called, returned, lin, this);
     invariant {:layer 1} (forall j: Invoc ::
-      hb(j, this) ==> Set_subset(vis[j], my_vis));
+      hb[j][this] ==> Set_subset(vis[j], my_vis));
     invariant {:layer 1} (forall n1: Invoc :: {my_vis[n1]}
       my_vis[n1] ==> Set_ofSeq(lin)[n1]);
     invariant {:layer 1} known(c) && (usedFP[c] || queueFP[c]);
@@ -693,9 +702,9 @@ procedure {:yields} {:layer 1} {:refines "size_atomic"} size({:linear "this"} th
       ==> s == ci - 1 - Queue.stateHead(Queue.ofSeq(Seq_restr(lin, my_vis)));
 
     yield;
-    assert {:layer 1} Inv(queueFP, usedFP, start, head, tail, next, data, nextTags, nextInvoc, nextRef, lin, vis, absRefs, called, returned) && preLP(called, returned, lin, this);
+    assert {:layer 1} Inv(queueFP, usedFP, start, head, tail, next, data, nextTags, nextInvoc, nextRef, hb, lin, vis, absRefs, called, returned) && preLP(called, returned, lin, this);
     assert {:layer 1} (forall j: Invoc ::
-      hb(j, this) ==> Set_subset(vis[j], my_vis));
+      hb[j][this] ==> Set_subset(vis[j], my_vis));
     assert {:layer 1} (forall n1: Invoc :: {my_vis[n1]}
       my_vis[n1] ==> Set_ofSeq(lin)[n1]);
     assert {:layer 1} known(c) && (usedFP[c] || queueFP[c]);
@@ -727,22 +736,22 @@ procedure {:yields} {:layer 1} {:refines "size_atomic"} size({:linear "this"} th
   call intro_writeVis(this, my_vis);
 
   yield;
-  assert {:layer 1} Inv(queueFP, usedFP, start, head, tail, next, data, nextTags, nextInvoc, nextRef, lin, vis, absRefs, called, returned) && postLP(called, returned, lin, this);
+  assert {:layer 1} Inv(queueFP, usedFP, start, head, tail, next, data, nextTags, nextInvoc, nextRef, hb, lin, vis, absRefs, called, returned) && postLP(called, returned, lin, this);
   assert {:layer 1} (forall n1: Invoc :: {vis[this][n1]}
     vis[this][n1] ==> Set_ofSeq(lin)[n1]);
 }
 
 procedure {:yields} {:layer 1} {:refines "size_return_atomic"}
     size_return({:linear "this"} this: Invoc)
-  requires {:layer 1} Inv(queueFP, usedFP, start, head, tail, next, data, nextTags, nextInvoc, nextRef, lin, vis, absRefs, called, returned);
+  requires {:layer 1} Inv(queueFP, usedFP, start, head, tail, next, data, nextTags, nextInvoc, nextRef, hb, lin, vis, absRefs, called, returned);
   requires {:layer 1} postLP(called, returned, lin, this);
   requires {:layer 1} (forall n1: Invoc :: {vis[this][n1]}
     vis[this][n1] ==> Set_ofSeq(lin)[n1]);
-  ensures {:layer 1} Inv(queueFP, usedFP, start, head, tail, next, data, nextTags, nextInvoc, nextRef, lin, vis, absRefs, called, returned);
+  ensures {:layer 1} Inv(queueFP, usedFP, start, head, tail, next, data, nextTags, nextInvoc, nextRef, hb, lin, vis, absRefs, called, returned);
   modifies returned;
 {
   yield;
-  assert {:layer 1} Inv(queueFP, usedFP, start, head, tail, next, data, nextTags, nextInvoc, nextRef, lin, vis, absRefs, called, returned);
+  assert {:layer 1} Inv(queueFP, usedFP, start, head, tail, next, data, nextTags, nextInvoc, nextRef, hb, lin, vis, absRefs, called, returned);
   assert {:layer 1} postLP(called, returned, lin, this);
   assert {:layer 1} (forall n1: Invoc :: {vis[this][n1]}
     vis[this][n1] ==> Set_ofSeq(lin)[n1]);
@@ -750,5 +759,5 @@ procedure {:yields} {:layer 1} {:refines "size_return_atomic"}
   call intro_writeReturned(this);
 
   yield;
-  assert {:layer 1} Inv(queueFP, usedFP, start, head, tail, next, data, nextTags, nextInvoc, nextRef, lin, vis, absRefs, called, returned);
+  assert {:layer 1} Inv(queueFP, usedFP, start, head, tail, next, data, nextTags, nextInvoc, nextRef, hb, lin, vis, absRefs, called, returned);
 }
